decidable equality for verse primitives

src/Verse/Language.v
@@ -2,9 +2,14 @@
 Require Import Verse.Types.
 Require Import Verse.Types.Internal.
 Require Import Verse.Syntax.
+
+Require Import Equality.
+Require Import Eqdep_dec.
 Require Import Bool.
 Require Import Omega.
 Require Import List.
+Import String.
+Import Nat.
 Import ListNotations.
 
 (* end hide *)
@@ -67,7 +72,58 @@ Section Language.
   Definition larg := arg lval.
   Definition rarg := arg rval.
 
+  Let directarg := sigT (arg direct).
+  
+  Variable v_eq_dec : forall {k} {ty : type k} (v1 v2 : v _ ty), {v1 = v2} + {v1 <> v2}.
 
+  Arguments v_eq_dec [k ty] _.
+
+  Lemma exists_eq_dec T (T_dec : forall (a b : T), {a = b} + {a <> b})
+                   (P : T -> Prop)
+                   (P_eq_dec : forall (t : T) (p q : P t), {p = q} + {p <> q}) :
+                   forall (p1 p2 : {t : T | P t}), {p1 = p2} + {p1 <> p2}.
+  Proof.
+    Set Keep Proof Equalities.
+    destruct p1. destruct p2.
+    destruct (T_dec x x0). subst. destruct (P_eq_dec _ p p0). subst p0.
+    - left; trivial.
+    - right; unfold not; intros; injection H; 
+        intros; inversion_sigma;
+        pose (eq_rect_eq_dec T_dec (fun a : T => P a) p H1);
+            rewrite <- e in H2; contradiction.
+    - right; congruence.
+      Unset Keep Proof Equalities.
+  Qed.
+
+  Axiom lt_unique : forall n m (p q : n < m), p = q.
+  Definition lt_eq_dec n m (p q : n < m) : {p = q} + {p <> q} := left (lt_unique n m p q).
+
+  Lemma arg_eq_dec : forall (a1 a2 : {ty : type direct & arg _ ty}), {a1 = a2} + {a1 <> a2}.
+    destruct a1, a2.
+    dependent destruction a; dependent destruction a0;
+      try (solve [(right; unfold not; inversion 1)]).
+    * destruct (ty_eq_dec x x0); subst; [ | right ; unfold not; inversion 1; contradiction ..].
+      destruct (v_eq_dec v0 v1); [left; congruence | right]; 
+        unfold not; inversion 1.
+      pose (inj_pair2_eq_dec _ ty_eq_dec _ _ _ _ H1); contradiction.
+    * destruct (ty_eq_dec x x0); subst; [ | right ; unfold not; inversion 1; contradiction ..].
+      destruct (constant_dec x0 c c0); [left; congruence | right];
+        unfold not; inversion 1.
+      pose (inj_pair2_eq_dec _ ty_eq_dec _ _ _ _ H1).
+      contradiction.
+    * destruct (ty_eq_dec x x0); destruct (eq_dec b b0);
+        destruct (endian_eq_dec e e0); destruct (ty_eq_dec x x0);
+          subst; [ | right; unfold not; inversion 1; contradiction ..].
+      destruct (v_eq_dec v0 v1).
+      destruct (exists_eq_dec _ eq_dec _ (fun n => lt_eq_dec n b0) s s0);
+        [ left; congruence | right ].
+      unfold not; inversion 1.
+      pose (inj_pair2_eq_dec _ eq_dec _ _ _ _ H2); contradiction.
+      right; unfold not; inversion 1.
+      pose (inj_pair2_eq_dec _ eq_dec _ _ _ _ H1).
+      pose (inj_pair2_eq_dec _ endian_eq_dec _ _ _ _ e).
+      pose (inj_pair2_eq_dec _ ty_eq_dec _ _ _ _ e1); contradiction.
+  Defined.        
 
   (** ** Assignment statement.
 
@@ -146,6 +202,7 @@ program block is merely a list of instructions.
 End Language.
 
 Arguments Indices [v a b e ty] _.
+
 
 (**
 
