src/Verse/Word.v
@@ -4,11 +4,13 @@ Require Import Verse.Error.
 Require Import Vector.
 Require Import Coq.NArith.Ndigits.
 Require Import BinNums.
-Require Import BigNumPrelude.
+
 Require Import String.
 Require Import Ascii.
 Require Import Verse.PrettyPrint.
 Local Open Scope N_scope.
+
+Require Import Verse.DecFacts.
 (* end hide *)
 
 (** * Words.
@@ -28,9 +30,17 @@ Arguments bits [n] _.
 (** Words measured in units of bytes *)
 Definition bytes n := t (8 * n).
 
-
 (* Errors while encoding *)
 Inductive EncodeError : Prop := BadBase16 | BadBinary | TooFewDigits | TooManyDigits.
+
+Lemma bytes_dec : forall (n : nat) (a b : bytes n), {a = b} + {a <> b}.
+  unfold bytes. destruct a. destruct b0. 
+  unfold Bvector.Bvector in b, b0.
+  pose (vec_eq_dec bool bool_dec (8 * n) b b0).
+  destruct s.
+  left; apply f_equal; trivial.
+  right; unfold not; inversion 1; contradiction.
+Qed.
 
 (* begin hide *)
 Definition toN {n}(x : t n) :=
